[MERGE] Duplicate Register Removal
commit 63ee2ba3223c1361cd30da1b9f3b57fd6cba1a54
Author: Basile Pesin <basile.pesin@vertmo.org>
Date:   Fri Jun 18 18:24:41 2021 +0200

    Simplified expression explicitation and related proofs

commit 698ae22cabb746c93262f2e81d8bfe7322390e5a
Author: Basile Pesin <basile.pesin@vertmo.org>
Date:   Fri Jun 18 13:51:45 2021 +0200

    Preservation of semantics through DRR

commit da7ccbd081483fb35bcdf350c342cef7c8b5fca2
Author: Basile Pesin <basile.pesin@vertmo.org>
Date:   Thu Jun 17 18:34:31 2021 +0200

    Preservation of static properties through DRR

commit 9a66f1cfdd98be96dd436c30c91be4c73a560278
Author: Basile Pesin <basile.pesin@vertmo.org>
Date:   Tue Jun 15 21:15:39 2021 +0200

    Moved DupRegRem.v to its own folder in preparation of the proofs to come

commit 2cd275747206f414615add4191ced331fe747c33
Author: Basile Pesin <basile.pesin@vertmo.org>
Date:   Tue Jun 15 19:35:10 2021 +0200

    Fixed an error and solved the nodes obligations

commit cecf19c2f858082b7e774ce2e17883ca16af9ca5
Author: Basile Pesin <basile.pesin@vertmo.org>
Date:   Mon Jun 14 15:18:02 2021 +0200

    Algorithm for removal of duplicate registers

src/veluslib.ml
@@ -10,6 +10,9 @@ let sync_destination = ref (None : string option)
 let main_node = ref (None : string option)
 let reaction_counter = Camlcoq.intern_string "$reaction"
 
+let dupregrem = ref true
+let do_dupregrem () = !dupregrem
+
 let fuse_obc = ref true
 let do_fusion () = !fuse_obc
 
