extraction/Extraction.v
@@ -154,6 +154,7 @@ Extract Constant Velus.print_nlustre =>
 Extract Constant Velus.print_stc => "Veluslib.print_stc_if".
 Extract Constant Velus.print_sch => "Veluslib.print_sch_if".
 Extract Constant Velus.print_obc => "Veluslib.print_obc_if".
+Extract Constant Velus.do_dupregrem => "Veluslib.do_dupregrem".
 Extract Constant Velus.do_fusion => "Veluslib.do_fusion".
 Extract Constant Velus.do_norm_switches => "Veluslib.do_normalize_switches".
 Extract Constant Velus.do_sync   => "Veluslib.do_sync".
