src/NLustre/DupRegRem/DRRClocking.v
@@ -1,0 +1,376 @@
+From Coq Require Import List.
+Import List.ListNotations.
+Open Scope list_scope.
+
+From Coq Require Import Recdef.
+From Velus Require Import Common.
+From Velus Require Import CommonProgram.
+From Velus Require Import Operators.
+From Velus Require Import Clocks.
+From Velus Require Import Environment.
+From Velus Require Import CoreExpr.CESyntax.
+From Velus Require Import CoreExpr.CEClocking.
+From Velus Require Import NLustre.NLSyntax.
+From Velus Require Import NLustre.Memories.
+From Velus Require Import NLustre.IsDefined.
+From Velus Require Import NLustre.NLClocking.
+From Velus Require Import NLustre.NLOrdered.
+From Velus Require Import NLustre.DupRegRem.DupRegRem.
+
+Module Type DRRCLOCKING
+       (Import Ids   : IDS)
+       (Import Op    : OPERATORS)
+       (Import OpAux : OPERATORS_AUX   Ids Op)
+       (Import Cks   : CLOCKS          Ids Op OpAux)
+       (Import CESyn : CESYNTAX        Ids Op OpAux Cks)
+       (Import CEClo : CECLOCKING      Ids Op OpAux Cks CESyn)
+       (Import Syn   : NLSYNTAX        Ids Op OpAux Cks CESyn)
+       (Import Ord   : NLORDERED       Ids Op OpAux Cks CESyn Syn)
+       (Import Mem   : MEMORIES        Ids Op OpAux Cks CESyn Syn)
+       (Import IsD   : ISDEFINED       Ids Op OpAux Cks CESyn Syn Mem)
+       (Import Clo   : NLCLOCKING      Ids Op OpAux Cks CESyn Syn Ord Mem IsD CEClo)
+       (Import DRR   : DUPREGREM       Ids Op OpAux Cks CESyn Syn).
+
+  Section substitute.
+    Variable sub : Env.t ident.
+
+    Variable inouts : list (ident * clock).
+    Variable vars vars' : list (ident * clock).
+
+    Hypothesis Hsub : forall x y ck,
+        Env.find x sub = Some y ->
+        In (x, ck) (inouts ++ vars) ->
+        In (y, subst_in_clock sub ck) (inouts ++ vars').
+
+    Hypothesis Hnsub : forall x ck,
+        Env.find x sub = None ->
+        In (x, ck) (inouts ++ vars) ->
+        In (x, subst_in_clock sub ck) (inouts ++ vars').
+
+    Lemma subst_in_var_wc : forall x ck,
+        In (x, ck) (inouts ++ vars) ->
+        In (subst_in_var sub x, subst_in_clock sub ck) (inouts ++ vars').
+    Proof.
+      intros * Hin.
+      unfold subst_in_var.
+      destruct (Env.find _ _) eqn:Hfind; eauto.
+    Qed.
+
+    Variable (G : global).
+
+    Lemma subst_in_clock_wc : forall ck,
+        wc_clock (inouts ++ vars) ck ->
+        wc_clock (inouts ++ vars') (subst_in_clock sub ck).
+    Proof.
+      induction ck; intros * Hwc; inv Hwc; auto.
+      simpl. constructor; eauto using subst_in_var_wc.
+    Qed.
+
+    Lemma subst_in_exp_wc : forall e ck,
+        wc_exp (inouts ++ vars) e ck ->
+        wc_exp (inouts ++ vars') (subst_in_exp sub e) (subst_in_clock sub ck).
+    Proof.
+      intros * Hwc; induction Hwc;
+        simpl; econstructor; eauto using subst_in_var_wc.
+    Qed.
+
+    Lemma subst_in_cexp_wc : forall e ck,
+        wc_cexp (inouts ++ vars) e ck ->
+        wc_cexp (inouts ++ vars') (subst_in_cexp sub e) (subst_in_clock sub ck).
+    Proof.
+      induction e using cexp_ind2'; intros * Hwc; inv Hwc;
+        simpl; econstructor; eauto using subst_in_var_wc, subst_in_exp_wc.
+      - contradict H5.
+        eapply map_eq_nil; eauto.
+      - rewrite map_length, Forall2_map_2.
+        eapply Forall2_impl_In; [|eauto]; intros; simpl in *.
+        eapply Forall_forall in H; eauto. eapply H in H2; eauto.
+      - contradict H4.
+        eapply map_eq_nil; eauto.
+      - intros ? Hin.
+        eapply in_map_iff in Hin as (?&Hopt&Hin).
+        eapply option_map_inv in Hopt as (?&?&?); subst.
+        eapply Forall_forall in H; eauto. simpl in *.
+        eapply H in H7; eauto.
+    Qed.
+
+    Lemma instck_subst_in_clock : forall ck sub0 bck ck',
+      instck bck sub0 ck = Some ck' ->
+      instck (subst_in_clock sub bck) (fun x => option_map (fun x1 => subst_in_var sub x1) (sub0 x)) ck =
+      Some (subst_in_clock sub ck').
+    Proof.
+      induction ck; intros * Hinst1; simpl in *.
+      - inv Hinst1; auto.
+      - destruct (instck bck sub0 ck) eqn:Hinst. 2:inv Hinst1.
+        eapply IHck in Hinst. rewrite Hinst.
+        destruct (sub0 i); inv Hinst1; simpl. reflexivity.
+    Qed.
+
+    Hint Resolve subst_in_var_wc subst_in_clock_wc subst_in_exp_wc subst_in_cexp_wc.
+
+    Lemma subst_in_equation_wc : forall equ,
+        (forall x, In x (var_defined equ) -> Env.find x sub = None) ->
+        wc_equation G (inouts ++ vars) equ ->
+        wc_equation G (inouts ++ vars') (subst_in_equation sub equ).
+    Proof.
+      intros * Hdef Hwc; inv Hwc; simpl in *.
+      - constructor; eauto.
+      - eapply CEqApp with (sub:=fun x => option_map (fun x => subst_in_var sub x) (sub0 x)) (* ? *); eauto.
+        + rewrite Forall2_map_2. eapply Forall2_impl_In; [|eauto]; intros (?&?&?) ? _ _ (?&?&?&?).
+          repeat (esplit; eauto).
+          * inv H3; simpl; constructor.
+          * apply instck_subst_in_clock; auto.
+        + eapply Forall2_impl_In; [|eauto]; intros (?&?&?) ? _ Hin2 (?&?&?&?).
+          repeat (esplit; eauto).
+          * rewrite H3; simpl.
+            unfold subst_in_var. rewrite Hdef; eauto.
+          * eapply instck_subst_in_clock; eauto.
+        + unfold subst_in_reset.
+          rewrite Forall_map. eapply Forall_impl; [|eauto]; intros (?&?) ?; eauto.
+      - constructor; auto.
+        unfold subst_in_reset.
+          rewrite Forall_map. eapply Forall_impl; [|eauto]; intros (?&?) ?; eauto.
+    Qed.
+
+  End substitute.
+
+  Lemma remove_dup_regs_once_wc : forall G inouts vars eqs,
+      NoDupMembers (inouts ++ idck vars) ->
+      NoDup (vars_defined eqs) ->
+      (forall x eq, In eq eqs -> In x (var_defined eq) -> is_fby eq = true -> ~InMembers x inouts) ->
+      wc_env inouts ->
+      Forall (wc_equation G (inouts ++ idck vars)) eqs ->
+      let (vars', eqs') := remove_dup_regs_eqs_once vars eqs in
+      Forall (wc_equation G (inouts ++ idck vars')) eqs'.
+  Proof.
+    intros * Hndv Hnd Hinouts Hwinouts Hwc.
+    destruct (remove_dup_regs_eqs_once _ _) eqn:Honce. inv Honce.
+    unfold subst_and_filter_equations.
+    rewrite Forall_map, Forall_filter. eapply Forall_impl_In; eauto.
+    intros ? Hineq Hwc' Hfilter.
+    eapply subst_in_equation_wc; [| | |eauto].
+    - intros * Hfind Hin.
+      assert (~InMembers x inouts) as Hnx.
+      { apply find_duplicates_spec in Hfind as (?&?&?&?&?&Hin1&_&_).
+        eapply Hinouts in Hin1; eauto. simpl; auto. }
+      assert (~InMembers y inouts) as Hny.
+      { apply find_duplicates_spec in Hfind as (?&?&?&?&?&_&Hin2&_).
+        eapply Hinouts in Hin2; eauto. simpl; auto. }
+      rewrite in_app_iff in *. destruct Hin as [Hin|Hin].
+      1:(exfalso; eauto using In_InMembers).
+      right.
+      rewrite In_idck_exists in *. destruct Hin as (?&Hin).
+      assert (Hfind':=Hfind).
+      eapply find_duplicates_spec in Hfind as (?&?&?&?&?&Hwt1&Hwt2&_).
+      eapply Forall_forall in Hwt1; eauto. eapply Forall_forall in Hwt2; eauto.
+      inv Hwt1. inv Hwt2.
+      rewrite in_app_iff in H2, H3.
+      destruct H2 as [Hin1|Hin1], H3 as [Hin2|Hin2].
+      1-3:(exfalso; eauto using In_InMembers).
+      eapply In_idck_exists in Hin1 as (?&Hin1).
+      eapply In_idck_exists in Hin2 as (ty&Hin2).
+      eapply NoDupMembers_det in Hin; eauto. 2:eapply NoDupMembers_app_r, NoDupMembers_idck in Hndv; eauto.
+      inv Hin. exists ty; simpl.
+      eapply in_map_iff. exists (y, (ty, ck)); split; auto.
+      eapply filter_In; split; auto.
+       eapply find_duplicates_irrefl in Hfind'; eauto.
+       apply Env.Props.P.F.not_mem_in_iff in Hfind'. rewrite Hfind'; auto.
+    - intros * Hfind Hin.
+      rewrite in_app_iff in *. destruct Hin as [Hin|Hin]; auto.
+      + assert (forall x, Env.In x (find_duplicates eqs) -> ~InMembers x inouts) as Hninouts.
+        { clear Hfind. intros ? Hindup.
+          rewrite Env.In_find in Hindup. destruct Hindup as (?&Hfind).
+          eapply find_duplicates_spec in Hfind as (?&?&?&?&?&Hin1&_).
+          eapply Hinouts; eauto. simpl; auto.
+        }
+        assert (subst_in_clock (find_duplicates eqs) ck = ck); repeat rewrite H; auto.
+        eapply wc_env_var in Hin; eauto.
+        clear - Hin Hwinouts Hninouts.
+        induction Hin; simpl; auto.
+        f_equal; auto.
+        unfold subst_in_var. destruct (Env.find _ _) eqn:Hfind; auto.
+        apply Env.find_In, Hninouts in Hfind.
+        exfalso; eauto using In_InMembers.
+      + right.
+        rewrite In_idck_exists in *. destruct Hin as (ty&Hin).
+        exists ty.
+        apply in_map_iff. exists (x, (ty, ck)); split; auto.
+        apply filter_In; split; auto.
+        rewrite Env.mem_find, Hfind; auto.
+    - intros * Hindef.
+      destruct (Env.find _ _) eqn:Hfind; auto. exfalso.
+      apply Env.find_In in Hfind.
+      assert (Hisfby:=Hindef). eapply find_duplicates_is_fby in Hisfby; eauto.
+      destruct a; simpl in *; try congruence.
+      inv Hindef; auto.
+      rewrite Bool.negb_true_iff, <-Env.Props.P.F.not_mem_in_iff in Hfilter.
+      congruence.
+  Qed.
+
+  Lemma remove_dup_regs_once_wc_env : forall G inouts vars eqs vars' eqs',
+      NoDupMembers (inouts ++ idck vars) ->
+      NoDup (vars_defined eqs) ->
+      (forall x eq, In eq eqs -> In x (var_defined eq) -> is_fby eq = true -> ~InMembers x inouts) ->
+      wc_env inouts ->
+      wc_env (inouts ++ idck vars) ->
+      Forall (wc_equation G (inouts ++ idck vars)) eqs ->
+      remove_dup_regs_eqs_once vars eqs = (vars', eqs') ->
+      wc_env (inouts ++ idck vars').
+  Proof.
+    intros * Hndv Hnd Hinouts Hwc1 Hwc2 Hwceq Hrem.
+    inv Hrem.
+    eapply Forall_app; split.
+    - eapply Forall_impl; [|eauto]; intros (?&?) ?.
+      eapply wc_clock_incl; eauto. apply incl_appl, incl_refl.
+    - eapply Forall_app in Hwc2 as (?&Hwc2).
+      unfold idck in *.
+      rewrite Forall_map in *. eapply Forall_map, Forall_filter.
+      eapply Forall_impl_In; [|eauto]. intros (?&?&?) ? Hwc Hmem; simpl in *.
+      eapply subst_in_clock_wc; eauto; intros * Hfind Hin.
+      + assert (~InMembers x inouts) as Hnx.
+        { apply find_duplicates_spec in Hfind as (?&?&?&?&?&Hin1&_&_).
+          eapply Hinouts in Hin1; eauto. simpl; auto. }
+        assert (~InMembers y inouts) as Hny.
+        { apply find_duplicates_spec in Hfind as (?&?&?&?&?&_&Hin2&_).
+          eapply Hinouts in Hin2; eauto. simpl; auto. }
+        rewrite in_app_iff in *. destruct Hin as [Hin|Hin].
+        1:(exfalso; eauto using In_InMembers).
+        right.
+        rewrite in_map_iff in *. destruct Hin as ((?&ty0&?)&Heq&Hin); inv Heq; simpl in *.
+        assert (Hfind':=Hfind).
+        eapply find_duplicates_spec in Hfind as (?&?&?&?&?&Hwt1&Hwt2&_).
+        eapply Forall_forall in Hwt1; eauto. eapply Forall_forall in Hwt2; eauto.
+        inv Hwt1. inv Hwt2.
+        rewrite in_app_iff in H4, H5.
+        destruct H4 as [Hin1|Hin1], H5 as [Hin2|Hin2].
+        1-3:(exfalso; eauto using In_InMembers).
+        eapply In_idck_exists in Hin1 as (?&Hin1).
+        eapply In_idck_exists in Hin2 as (ty&Hin2).
+        eapply NoDupMembers_det in Hin; eauto. inv Hin. 2:eapply NoDupMembers_app_r, NoDupMembers_idck in Hndv; eauto.
+        exists (y, (ty, subst_in_clock (find_duplicates eqs) ck)); simpl; split; auto.
+        apply in_map_iff. exists (y, (ty, ck)); split; auto.
+        eapply filter_In; split; auto.
+        eapply find_duplicates_irrefl in Hfind'; eauto.
+        apply Env.Props.P.F.not_mem_in_iff in Hfind'. rewrite Hfind'; auto.
+      + rewrite in_app_iff in *. destruct Hin as [Hin|Hin]; auto.
+        * assert (forall x, Env.In x (find_duplicates eqs) -> ~InMembers x inouts) as Hninouts.
+          { clear Hfind. intros ? Hindup.
+            rewrite Env.In_find in Hindup. destruct Hindup as (?&Hfind).
+            eapply find_duplicates_spec in Hfind as (?&?&?&?&?&Hin1&_).
+            eapply Hinouts; eauto. simpl; auto.
+          }
+          assert (subst_in_clock (find_duplicates eqs) ck = ck) as Hck; repeat rewrite Hck; auto.
+          eapply wc_env_var in Hin; eauto.
+          clear - Hin Hwc1 Hninouts.
+          induction Hin; simpl; auto.
+          f_equal; auto.
+          unfold subst_in_var. destruct (Env.find _ _) eqn:Hfind; auto.
+          apply Env.find_In, Hninouts in Hfind.
+          exfalso; eauto using In_InMembers.
+        * right.
+          rewrite in_map_iff in *. destruct Hin as ((x0&ty0&ck0)&Heq&Hin); inv Heq; simpl in *.
+          exists (x, (ty0, subst_in_clock (find_duplicates eqs) ck)); simpl; split; auto.
+          apply in_map_iff. exists (x, (ty0, ck)); split; auto.
+          apply filter_In; split; auto.
+          rewrite Env.mem_find, Hfind; auto.
+  Qed.
+
+  Lemma remove_dup_regs_eqs_wc : forall G inouts vars eqs vars' eqs',
+      NoDupMembers (inouts ++ idck vars) ->
+      NoDup (vars_defined eqs) ->
+      (forall x eq, In eq eqs -> In x (var_defined eq) -> is_fby eq = true -> ~InMembers x inouts) ->
+      wc_env inouts ->
+      wc_env (inouts ++ idck vars) ->
+      Forall (wc_equation G (inouts ++ idck vars)) eqs ->
+      remove_dup_regs_eqs vars eqs = (vars', eqs') ->
+      Forall (wc_equation G (inouts ++ idck vars')) eqs' /\ wc_env (inouts ++ idck vars').
+  Proof.
+    intros until eqs.
+    functional induction (remove_dup_regs_eqs vars eqs); intros * Hndv Hnd Hinouts Hwinouts Hwenv Hwc Hrem.
+    - eapply remove_dup_regs_once_wc_env in Hwenv; eauto.
+      eapply remove_dup_regs_once_wc in Hwc; eauto.
+      rewrite e in Hwc. inv e.
+      eapply IHp; eauto using subst_and_filter_equations_NoDup.
+      + clear - Hndv.
+        apply NoDupMembers_app; eauto using NoDupMembers_app_l.
+        * apply NoDupMembers_app_r, NoDupMembers_idck in Hndv.
+          apply NoDupMembers_idck, subst_and_filter_vars_NoDupMembers; auto.
+        * intros ? Hin.
+          eapply NoDupMembers_app_InMembers in Hndv; eauto.
+          contradict Hndv.
+          rewrite InMembers_idck in *; eauto using subst_and_filter_vars_InMembers.
+      + intros ?? Hin1 Hin2 Hisfby.
+        eapply in_map_iff in Hin1 as (?&?&Hin1); subst. apply in_filter in Hin1.
+        destruct x0; simpl in *; try congruence. destruct Hin2 as [Hin2|Hin2]; inv Hin2.
+        eapply Hinouts; eauto. simpl; auto.
+    - inv Hrem; auto.
+  Qed.
+
+  Lemma remove_dup_regs_node_wc : forall G n,
+      wc_node G n ->
+      wc_node (remove_dup_regs G) (remove_dup_regs_node n).
+  Proof.
+    intros * (Hwci&Hwco&Hwcv&Hwceq).
+    destruct (remove_dup_regs_eqs (n_vars n) (n_eqs n)) as (vars'&eqs') eqn:Hrem.
+    destruct (remove_dup_regs_eqs_wc G (idck (n_in n ++ n_out n)) (n_vars n) (n_eqs n) vars' eqs')
+      as (Hwc'&Hwenv'); eauto.
+    - rewrite <-idck_app, <-app_assoc, (Permutation.Permutation_app_comm (n_out _)).
+      apply NoDupMembers_idck, n_nodup.
+    - apply NoDup_var_defined_n_eqs.
+    - intros. intros contra. rewrite idck_app, InMembers_app in contra. destruct contra as [contra|contra].
+      + rewrite InMembers_idck in contra.
+        assert (In x (vars_defined (n_eqs n))) as Hdef.
+        { unfold vars_defined. apply in_flat_map.
+          eexists; split; eauto. }
+        rewrite n_defd in Hdef. apply fst_InMembers in Hdef.
+        eapply NoDupMembers_app_InMembers in contra. eapply contra; eauto.
+        eapply n_nodup.
+      + rewrite fst_InMembers, map_fst_idck in contra.
+        apply n_vout in contra. apply contra.
+        unfold vars_defined. apply in_flat_map.
+        eexists; split; eauto.
+        apply filter_In; auto.
+    - rewrite <-idck_app, <-app_assoc, (Permutation.Permutation_app_comm (n_out _)); auto.
+    - eapply Forall_impl; [|eauto]. intros ? Hwt.
+      eapply wc_equation_incl; eauto. clear -n. intros (?&?) Hin.
+      rewrite <-idck_app, <-app_assoc, (Permutation.Permutation_app_comm (n_out _)).
+      assumption.
+    - split; [|split; [|split]]; simpl; auto.
+      1,2:rewrite Hrem.
+      + simpl. rewrite <-idck_app, <-app_assoc, (Permutation.Permutation_app_comm (n_out _)) in Hwenv'; auto.
+      + eapply Forall_impl; [|eauto]. intros ? Hwt.
+        eapply global_iface_eq_wc_eq; eauto using remove_dup_regs_iface_eq.
+        eapply wc_equation_incl; eauto. clear -n. intros ? Hin.
+        repeat rewrite idck_app in *. repeat rewrite <-filter_app in Hin.
+        repeat rewrite in_app_iff in *.
+        destruct Hin as [[Hin|Hin]|Hin]; auto.
+  Qed.
+
+  Theorem remove_dup_regs_wc : forall G,
+      wc_global G ->
+      wc_global (remove_dup_regs G).
+  Proof.
+    intros.
+    unfold wc_global in *; simpl.
+    induction H; simpl; constructor; auto.
+    eapply remove_dup_regs_node_wc in H; auto.
+  Qed.
+
+End DRRCLOCKING.
+
+Module DrrClockingFun
+       (Ids   : IDS)
+       (Op    : OPERATORS)
+       (OpAux : OPERATORS_AUX   Ids Op)
+       (Cks   : CLOCKS          Ids Op OpAux)
+       (CESyn : CESYNTAX        Ids Op OpAux Cks)
+       (CEClo : CECLOCKING      Ids Op OpAux Cks CESyn)
+       (Syn   : NLSYNTAX        Ids Op OpAux Cks CESyn)
+       (Ord   : NLORDERED       Ids Op OpAux Cks CESyn Syn)
+       (Mem   : MEMORIES        Ids Op OpAux Cks CESyn Syn)
+       (IsD   : ISDEFINED       Ids Op OpAux Cks CESyn Syn Mem)
+       (Clo   : NLCLOCKING      Ids Op OpAux Cks CESyn Syn Ord Mem IsD CEClo)
+       (DRR   : DUPREGREM       Ids Op OpAux Cks CESyn Syn)
+  <: DRRCLOCKING Ids Op OpAux Cks CESyn CEClo Syn Ord Mem IsD Clo DRR.
+  Include DRRCLOCKING Ids Op OpAux Cks CESyn CEClo Syn Ord Mem IsD Clo DRR.
+End DrrClockingFun.
