src/NLustre/DupRegRem/DRRCorrectness.v
@@ -1,0 +1,389 @@
+From Coq Require Import List.
+Import List.ListNotations.
+Open Scope list_scope.
+
+From Coq Require Import Recdef.
+From Velus Require Import Common.
+From Velus Require Import CommonProgram.
+From Velus Require Import Operators.
+From Velus Require Import Clocks.
+From Velus Require Import Environment.
+From Velus Require Import IndexedStreams.
+From Velus Require Import CoreExpr.CESyntax.
+From Velus Require Import CoreExpr.CESemantics.
+From Velus Require Import NLustre.NLSyntax.
+From Velus Require Import NLustre.NLOrdered.
+From Velus Require Import NLustre.NLIndexedSemantics.
+From Velus Require Import NLustre.DupRegRem.DupRegRem.
+
+Module Type DRRCORRECTNESS
+       (Import Ids   : IDS)
+       (Import Op    : OPERATORS)
+       (Import OpAux : OPERATORS_AUX      Ids Op)
+       (Import Cks   : CLOCKS             Ids Op OpAux)
+       (Import Str   : INDEXEDSTREAMS     Ids Op OpAux Cks)
+       (Import CESyn : CESYNTAX           Ids Op OpAux Cks)
+       (Import CESem : CESEMANTICS        Ids Op OpAux Cks CESyn Str)
+       (Import Syn   : NLSYNTAX           Ids Op OpAux Cks CESyn)
+       (Import Ord   : NLORDERED          Ids Op OpAux Cks CESyn Syn)
+       (Import Sem   : NLINDEXEDSEMANTICS Ids Op OpAux Cks CESyn Syn Str Ord CESem)
+       (Import DRR   : DUPREGREM          Ids Op OpAux Cks CESyn Syn).
+
+  (** ** Preservation of Ordered_nodes *)
+
+  Lemma remove_dup_regs_eqs_Is_node_in : forall f vars eqs,
+    Is_node_in f (snd (remove_dup_regs_eqs vars eqs)) ->
+    Is_node_in f eqs.
+  Proof.
+    intros *.
+    functional induction (remove_dup_regs_eqs vars eqs); intros * Hin; auto.
+    apply IHp in Hin. clear IHp.
+    inv e. clear - Hin. revert Hin. generalize (find_duplicates eqs); intros.
+    unfold subst_and_filter_equations, Is_node_in in *.
+    rewrite Exists_map in Hin.
+    induction eqs as [|[| |]]; simpl in *; auto.
+    - inv Hin.
+    - inv Hin; auto. inv H0.
+    - inv Hin; auto.
+      inv H0; auto. left. constructor.
+    - destruct (negb _); auto.
+      inv Hin; auto. inv H0.
+  Qed.
+
+  Theorem remove_dup_regs_Ordered : forall G,
+    Ordered_nodes G ->
+    Ordered_nodes (remove_dup_regs G).
+  Proof.
+    intros * Hord.
+    eapply transform_units_Ordered_program; eauto.
+    intros * Hin; simpl in *.
+    eapply remove_dup_regs_eqs_Is_node_in; eauto.
+  Qed.
+
+  (** ** Preservation of semantics *)
+
+  Section substitute_instant.
+
+    Variable (sub : Env.t ident).
+    Variable (base : bool).
+    Variable (R : env).
+
+    Hypothesis Hsub : forall x y,
+        Env.find x sub = Some y ->
+        Env.find x R = Env.find y R.
+
+    Lemma subst_sem_var_instant : forall x v,
+        sem_var_instant R x v <->
+        sem_var_instant R (subst_in_var sub x) v.
+    Proof.
+      intros *.
+      unfold subst_in_var, sem_var_instant.
+      destruct (Env.find x sub) eqn:Hfind; try reflexivity.
+      apply Hsub in Hfind. now rewrite Hfind.
+    Qed.
+    Hint Resolve subst_sem_var_instant.
+
+    Lemma subst_sem_clock_instant : forall ck v,
+        sem_clock_instant base R ck v <->
+        sem_clock_instant base R (subst_in_clock sub ck) v.
+    Proof.
+      split; revert v.
+      1,2:induction ck; intros * Hsem; simpl in *; inv Hsem.
+      1,5:constructor; auto.
+      1,4:eapply Son; eauto.
+      3,5:eapply Son_abs1; eauto.
+      5,6:eapply Son_abs2; eauto.
+      1,3,5:rewrite <-subst_sem_var_instant; auto.
+      1-3:apply subst_sem_var_instant; auto.
+    Qed.
+    Hint Resolve subst_sem_clock_instant.
+
+    Lemma subst_sem_clocked_var_instant : forall x ck,
+        sem_clocked_var_instant base R x ck ->
+        sem_clocked_var_instant base R (subst_in_var sub x) (subst_in_clock sub ck).
+    Proof.
+      intros * Hsem; inv Hsem.
+      rewrite subst_sem_clock_instant in *.
+      rewrite subst_sem_var_instant in *. setoid_rewrite subst_sem_var_instant in H.
+      constructor; auto.
+    Qed.
+
+    Corollary subst_sem_clocked_vars_instant : forall xcks,
+        sem_clocked_vars_instant base R xcks ->
+        sem_clocked_vars_instant base R (subst_in_reset sub xcks).
+    Proof.
+      unfold subst_in_reset, sem_clocked_vars_instant.
+      intros * Hsem.
+      rewrite Forall_map.
+      eapply Forall_impl; [|eauto]; intros (?&?) ?.
+      eapply subst_sem_clocked_var_instant; eauto.
+    Qed.
+
+    Lemma subst_sem_exp_instant : forall e v,
+        sem_exp_instant base R e v ->
+        sem_exp_instant base R (subst_in_exp sub e) v.
+    Proof.
+      induction e; intros * Hsem; simpl; auto.
+      - (* var *)
+        inv Hsem. constructor. rewrite <-subst_sem_var_instant; auto.
+      - (* when *)
+        inv Hsem.
+        + apply Swhen_eq; auto.
+          rewrite <-subst_sem_var_instant; auto.
+        + eapply Swhen_abs1; eauto.
+          rewrite <-subst_sem_var_instant; auto.
+        + eapply Swhen_abs; eauto.
+          rewrite <-subst_sem_var_instant; auto.
+      - (* unop *)
+        inv Hsem; econstructor; eauto.
+        rewrite subst_in_exp_typeof; auto.
+      - (* binop *)
+        inv Hsem; econstructor; eauto.
+        rewrite 2 subst_in_exp_typeof; auto.
+    Qed.
+    Hint Resolve subst_sem_exp_instant.
+
+    Corollary subst_sem_aexp_instant : forall ck e v,
+        sem_aexp_instant base R ck e v ->
+        sem_aexp_instant base R (subst_in_clock sub ck) (subst_in_exp sub e) v.
+    Proof.
+      intros * Hsem; inv Hsem.
+      1,2:constructor; auto; rewrite <-subst_sem_clock_instant; auto.
+    Qed.
+
+    Corollary subst_sem_exps_instant : forall es vs,
+        sem_exps_instant base R es vs ->
+        sem_exps_instant base R (map (subst_in_exp sub) es) vs.
+    Proof.
+      unfold sem_exps_instant.
+      intros * Hsem.
+      rewrite Forall2_map_1.
+      eapply Forall2_impl_In; [|eauto]; intros; eauto.
+    Qed.
+
+    Lemma subst_sem_cexp_instant : forall e v,
+        sem_cexp_instant base R e v ->
+        sem_cexp_instant base R (subst_in_cexp sub e) v.
+    Proof.
+      induction e using cexp_ind2'; intros * Hsem; simpl; auto.
+      - (* merge *)
+        destruct x; simpl.
+        inv Hsem; econstructor.
+        2:rewrite map_app; simpl; auto.
+        1-6:eauto.
+        1,4:rewrite <-subst_sem_var_instant; auto.
+        + now rewrite map_length.
+        + apply Forall_app in H as (_&Hf). inv Hf; auto.
+        + rewrite <-map_app, Forall_map.
+          eapply Forall_impl_In; [|eauto]; intros; simpl in *.
+          eapply Forall_forall with (x:=a) in H. 2:rewrite in_app_iff in *; simpl; destruct H0; auto.
+          eauto.
+        + rewrite Forall_map.
+          eapply Forall_impl_In; [|eapply H6]; intros. eapply Forall_forall in H; eauto.
+      - (* case *)
+        inv Hsem; econstructor; eauto.
+        + rewrite Forall2_map_1. eapply Forall2_impl_In; [|eauto]; intros.
+          eapply Forall_forall in H; eauto.
+          destruct a; simpl in *; auto.
+        + rewrite Forall_map. eapply Forall_impl_In; [|eauto]; intros.
+          eapply Forall_forall in H; eauto.
+          destruct a; simpl in *; eauto.
+      - (* eexp *)
+        inv Hsem. constructor; auto.
+    Qed.
+    Hint Resolve subst_sem_cexp_instant.
+
+    Corollary subst_sem_caexp_instant : forall ck e v,
+        sem_caexp_instant base R ck e v ->
+        sem_caexp_instant base R (subst_in_clock sub ck) (subst_in_cexp sub e) v.
+    Proof.
+      intros * Hsem; inv Hsem.
+      1,2:constructor; auto; rewrite <-subst_sem_clock_instant; auto.
+    Qed.
+
+  End substitute_instant.
+
+  Section substitute.
+    Variable (sub : Env.t ident).
+
+    Variable (G : global).
+    Variable (base : cstream).
+    Variable (H : history).
+
+    Hypothesis Hsub : forall x y,
+        Env.find x sub = Some y ->
+        forall n, Env.find x (H n) = Env.find y (H n).
+
+    Lemma subst_sem_var : forall x vs,
+        sem_var H x vs ->
+        sem_var H (subst_in_var sub x) vs.
+    Proof.
+      intros * Hsem ?.
+      rewrite <-subst_sem_var_instant; eauto.
+    Qed.
+
+    Lemma subst_sem_clock : forall ck vs,
+        sem_clock base H ck vs ->
+        sem_clock base H (subst_in_clock sub ck) vs.
+    Proof.
+      intros * Hsem ?.
+      rewrite <-subst_sem_clock_instant; eauto.
+    Qed.
+
+    Lemma subst_sem_equation : forall equ,
+        sem_equation G base H equ ->
+        sem_equation G base H (subst_in_equation sub equ).
+    Proof.
+      intros * Hsem; inv Hsem; simpl.
+      - (* def *)
+        econstructor; eauto using subst_sem_var.
+        intros ?; eapply subst_sem_caexp_instant; eauto.
+      - (* app *)
+        econstructor; eauto using subst_sem_clock.
+        + intros ?; eapply subst_sem_exps_instant; eauto.
+        + rewrite Forall2_map_1 in *.
+          unfold subst_in_reset. rewrite Forall2_map_1.
+          eapply Forall2_impl_In; [|eauto]; intros (?&?) ? _ _ ?; eauto using subst_sem_var.
+      - (* fby *)
+        econstructor; eauto.
+        + intros ?; eapply subst_sem_aexp_instant; eauto.
+        + rewrite Forall2_map_1 in *.
+          unfold subst_in_reset. rewrite Forall2_map_1.
+          eapply Forall2_impl_In; [|eauto]; intros (?&?) ? _ _ ?; eauto using subst_sem_var.
+        + intros ?. eapply subst_sem_clocked_vars_instant; eauto.
+    Qed.
+
+  End substitute.
+
+  Section remove_dup_regs_eqs.
+    Variable (G1 G2 : global).
+
+    Hypothesis Hglob : forall f ins outs,
+        sem_node G1 f ins outs -> sem_node G2 f ins outs.
+
+    Variable (base : cstream).
+    Variable (H : history).
+
+    Lemma Forall2_bools : forall H xs vs rs,
+        Forall2 (sem_var H) xs vs ->
+        bools_ofs vs rs ->
+        exists vs' , Forall2 (sem_var H) (PSP.to_list (PSP.of_list xs)) vs' /\
+                bools_ofs vs' rs.
+    Proof.
+      intros * Vars Bools; simpl.
+      assert (SameElements eq xs (PSP.to_list (PSP.of_list xs))) as Same.
+      { eapply ps_of_list_ps_to_list_SameElements; eauto. }
+      assert (Vars':=Vars). eapply @Forall2_SameElements_1 with (eqB:=eq) in Vars' as (vs'&Same'&?); eauto.
+      1-3:auto.
+      - rewrite Same' in Bools. eauto.
+      - intros * Eq1 Eq2 Var. rewrite <-Eq1, <-Eq2; auto.
+      - eauto using sem_var_det.
+    Qed.
+
+    Lemma ps_equal_Forall2_bools :
+      forall H xs ys vs vs' rs rs',
+        PS.Equal (PSP.of_list xs) (PSP.of_list ys) ->
+        Forall2 (sem_var H) xs vs ->
+        Forall2 (sem_var H) ys vs' ->
+        bools_ofs vs rs ->
+        bools_ofs vs' rs' ->
+        rs = rs'.
+    Proof.
+      intros * Eq Vars Vars' Bools Bools'.
+      assert (SameElements eq xs ys) as Same.
+      { eapply SE_trans. eapply ps_of_list_ps_to_list_SameElements.
+        symmetry. eapply SE_trans. eapply ps_of_list_ps_to_list_SameElements.
+        eapply SE_perm. rewrite <-Eq. reflexivity. }
+      eapply @Forall2_SameElements_1 with (eqB:=eq) in Vars as (vs''&Same'&Vars); eauto. 2:eauto.
+      assert (vs' = vs''); subst.
+      { eapply Forall2_swap_args in Vars'. eapply Forall2_trans_ex in Vars; eauto. clear - Vars.
+        induction Vars as [|???? (?&_&Hv1&Hv2)]; subst; auto.
+        eapply sem_var_det in Hv1; eauto; subst; auto. }
+      rewrite Same' in Bools.
+      eapply bools_ofs_det in Bools'; eauto.
+      - intros * Eq1 Eq2 Var. rewrite <-Eq1, <-Eq2; auto.
+      - eauto using sem_var_det.
+    Qed.
+
+    Lemma sem_EqFby_det : forall x y ck c0 e xr1 xr2,
+        PS.Equal (PSP.of_list (map fst xr1)) (PSP.of_list (map fst xr2)) ->
+        sem_equation G1 base H (EqFby x ck c0 e xr1) ->
+        sem_equation G1 base H (EqFby y ck c0 e xr2) ->
+        forall n, Env.find x (H n) = Env.find y (H n).
+    Proof.
+      intros * Heq Hsem1 Hsem2.
+      inv Hsem1. inv Hsem2.
+      eapply sem_aexp_det in H6; eauto; subst.
+      eapply ps_equal_Forall2_bools in H17; eauto; subst.
+      intros n. specialize (H9 n). specialize (H14 n).
+      rewrite H9, H14. reflexivity.
+    Qed.
+
+    Lemma remove_dup_regs_eqs_sem : forall vars eqs,
+        Forall (sem_equation G1 base H) eqs ->
+        Forall (sem_equation G2 base H) (snd (remove_dup_regs_eqs vars eqs)).
+    Proof.
+      intros * Hsem.
+      functional induction (remove_dup_regs_eqs vars eqs).
+      - apply IHp. clear IHp.
+        inv e.
+        unfold subst_and_filter_equations.
+        rewrite Forall_map, Forall_filter.
+        eapply Forall_impl; [|eauto]; intros * ? _.
+        eapply subst_sem_equation; eauto.
+        intros ?? Hfind.
+        eapply find_duplicates_spec in Hfind as (?&?&?&?&?&Hfby1&Hfby2&Heq).
+        eapply Forall_forall in Hfby1; eauto.
+        eapply Forall_forall in Hfby2; eauto.
+        eapply sem_EqFby_det; eauto.
+      - clear - Hglob Hsem.
+        eapply Forall_impl; [|eauto]; intros.
+        inv H0; econstructor; eauto.
+    Qed.
+
+  End remove_dup_regs_eqs.
+
+  Theorem remove_dup_regs_sem : forall G f ins outs,
+      Ordered_nodes G ->
+      sem_node G f ins outs ->
+      sem_node (remove_dup_regs G) f ins outs.
+  Proof.
+    intros (enms&nds).
+    unfold remove_dup_regs.
+    induction nds; intros * Hord Hsem; simpl; auto.
+    destruct (ident_eq_dec (n_name a) f).
+    - inv Hsem. rewrite find_node_now in H1; inv H1; auto.
+      econstructor; simpl; auto. rewrite find_node_now; eauto.
+      1-3:simpl; eauto.
+      eapply Forall_sem_equation_global_tl in H5; eauto.
+      2:{ eapply not_Is_called_in_self in Hord; eauto.
+          setoid_rewrite find_unit_now; eauto. simpl; eauto. }
+      eapply Forall_sem_equation_global_tl'; eauto.
+      1,2:eapply remove_dup_regs_Ordered in Hord; eauto.
+      { eapply not_Is_called_in_self in Hord; eauto.
+        setoid_rewrite find_unit_now; eauto. simpl; eauto. }
+      eapply remove_dup_regs_eqs_sem in H5; [simpl;eauto|].
+      inv Hord; eauto.
+    - eapply sem_node_cons in Hsem; eauto.
+      eapply sem_node_cons'; eauto.
+      + eapply remove_dup_regs_Ordered in Hord; eauto.
+      + inv Hord; eauto.
+  Qed.
+
+End DRRCORRECTNESS.
+
+Module DrrCorrectnessFun
+       (Ids   : IDS)
+       (Op    : OPERATORS)
+       (OpAux : OPERATORS_AUX      Ids Op)
+       (Cks   : CLOCKS             Ids Op OpAux)
+       (Str   : INDEXEDSTREAMS     Ids Op OpAux Cks)
+       (CESyn : CESYNTAX           Ids Op OpAux Cks)
+       (CESem : CESEMANTICS        Ids Op OpAux Cks CESyn Str)
+       (Syn   : NLSYNTAX           Ids Op OpAux Cks CESyn)
+       (Ord   : NLORDERED          Ids Op OpAux Cks CESyn Syn)
+       (Sem   : NLINDEXEDSEMANTICS Ids Op OpAux Cks CESyn Syn Str Ord CESem)
+       (DRR   : DUPREGREM          Ids Op OpAux Cks CESyn Syn)
+<: DRRCORRECTNESS Ids Op OpAux Cks Str CESyn CESem Syn Ord Sem DRR.
+  Include DRRCORRECTNESS Ids Op OpAux Cks Str CESyn CESem Syn Ord Sem DRR.
+End DrrCorrectnessFun.
