src/NLustre/DupRegRem/DRRNormalArgs.v
@@ -1,0 +1,102 @@
+From Coq Require Import List.
+Import List.ListNotations.
+Open Scope list_scope.
+
+From Coq Require Import Recdef.
+From Velus Require Import Common.
+From Velus Require Import CommonProgram.
+From Velus Require Import Operators.
+From Velus Require Import Clocks.
+From Velus Require Import Environment.
+From Velus Require Import CoreExpr.CESyntax.
+From Velus Require Import CoreExpr.CETyping.
+From Velus Require Import NLustre.NLSyntax.
+From Velus Require Import NLustre.NLTyping.
+From Velus Require Import NLustre.NLOrdered.
+From Velus Require Import NLustre.NLNormalArgs.
+From Velus Require Import NLustre.DupRegRem.DupRegRem.
+
+(** Remove duplicate registers in an NLustre program *)
+
+Module Type DRRNORMALARGS
+       (Import Ids   : IDS)
+       (Import Op    : OPERATORS)
+       (Import OpAux : OPERATORS_AUX   Ids Op)
+       (Import Cks   : CLOCKS          Ids Op OpAux)
+       (Import CESyn : CESYNTAX        Ids Op OpAux Cks)
+       (Import CETyp : CETYPING        Ids Op OpAux Cks CESyn)
+       (Import Syn   : NLSYNTAX        Ids Op OpAux Cks CESyn)
+       (Import Ord   : NLORDERED       Ids Op OpAux Cks CESyn Syn)
+       (Import Typ   : NLTYPING        Ids Op OpAux Cks CESyn Syn Ord CETyp)
+       (Import Norm  : NLNORMALARGS    Ids Op OpAux Cks CESyn CETyp Syn Ord Typ)
+       (Import DRR   : DUPREGREM       Ids Op OpAux Cks CESyn Syn).
+
+  Lemma subst_in_exp_noops_exp : forall sub e ck,
+    noops_exp ck e ->
+    noops_exp ck (subst_in_exp sub e).
+  Proof.
+    induction e; intros * Hnormed; simpl; auto.
+    1-4:destruct ck; simpl in *; auto.
+  Qed.
+
+  Lemma subst_in_equation_normal_args : forall G sub equ,
+    normal_args_eq G equ ->
+    normal_args_eq G (subst_in_equation sub equ).
+  Proof.
+    intros * Hnorm; inv Hnorm; simpl;
+      econstructor; eauto.
+    rewrite Forall2_map_2. eapply Forall2_impl_In; [|eauto]; intros.
+    apply subst_in_exp_noops_exp; auto.
+  Qed.
+
+  Lemma remove_dup_regs_normal_args_eqs : forall G sub eqs,
+      Forall (normal_args_eq G) eqs ->
+      Forall (normal_args_eq G) (snd (remove_dup_regs_eqs sub eqs)).
+  Proof.
+    intros * Hnormed.
+    functional induction (remove_dup_regs_eqs sub eqs); auto.
+    apply IHp.
+    inv e. unfold subst_and_filter_equations.
+    rewrite Forall_map, Forall_filter.
+    eapply Forall_impl; eauto; intros * Hn _.
+    eapply subst_in_equation_normal_args; eauto.
+  Qed.
+
+  Lemma remove_dup_regs_normal_args_node : forall G n,
+      normal_args_node G n ->
+      normal_args_node (remove_dup_regs G) (remove_dup_regs_node n).
+  Proof.
+    unfold normal_args_node.
+    intros * Hnormed; simpl.
+    apply remove_dup_regs_normal_args_eqs; auto.
+    eapply Forall_impl; [|eauto]. intros.
+    eapply global_iface_eq_normal_args_eq; eauto.
+    apply remove_dup_regs_iface_eq.
+  Qed.
+
+  Theorem remove_dup_regs_normal_args : forall G,
+      normal_args G ->
+      normal_args (remove_dup_regs G).
+  Proof.
+    unfold normal_args; simpl.
+    induction 1 as [|?? NAS]; simpl; constructor; auto.
+    apply remove_dup_regs_normal_args_node in NAS; auto.
+  Qed.
+
+End DRRNORMALARGS.
+
+Module DrrNormalArgsFun
+       (Ids   : IDS)
+       (Op    : OPERATORS)
+       (OpAux : OPERATORS_AUX   Ids Op)
+       (Cks   : CLOCKS          Ids Op OpAux)
+       (CESyn : CESYNTAX        Ids Op OpAux Cks)
+       (CETyp : CETYPING        Ids Op OpAux Cks CESyn)
+       (Syn   : NLSYNTAX        Ids Op OpAux Cks CESyn)
+       (Ord   : NLORDERED       Ids Op OpAux Cks CESyn Syn)
+       (Typ   : NLTYPING        Ids Op OpAux Cks CESyn Syn Ord CETyp)
+       (Norm  : NLNORMALARGS    Ids Op OpAux Cks CESyn CETyp Syn Ord Typ)
+       (DRR   : DUPREGREM       Ids Op OpAux Cks CESyn Syn)
+  <: DRRNORMALARGS Ids Op OpAux Cks CESyn CETyp Syn Ord Typ Norm DRR.
+  Include DRRNORMALARGS Ids Op OpAux Cks CESyn CETyp Syn Ord Typ Norm DRR.
+End DrrNormalArgsFun.
