src/NLustre/DupRegRem/DRRTyping.v
@@ -1,0 +1,294 @@
+From Coq Require Import List.
+Import List.ListNotations.
+Open Scope list_scope.
+
+From Coq Require Import Recdef.
+From Velus Require Import Common.
+From Velus Require Import CommonProgram.
+From Velus Require Import Operators.
+From Velus Require Import Clocks.
+From Velus Require Import Environment.
+From Velus Require Import CoreExpr.CESyntax.
+From Velus Require Import CoreExpr.CETyping.
+From Velus Require Import NLustre.NLSyntax.
+From Velus Require Import NLustre.NLTyping.
+From Velus Require Import NLustre.NLOrdered.
+From Velus Require Import NLustre.DupRegRem.DupRegRem.
+
+Module Type DRRTYPING
+       (Import Ids   : IDS)
+       (Import Op    : OPERATORS)
+       (Import OpAux : OPERATORS_AUX   Ids Op)
+       (Import Cks   : CLOCKS          Ids Op OpAux)
+       (Import CESyn : CESYNTAX        Ids Op OpAux Cks)
+       (Import CETyp : CETYPING        Ids Op OpAux Cks CESyn)
+       (Import Syn   : NLSYNTAX        Ids Op OpAux Cks CESyn)
+       (Import Ord   : NLORDERED       Ids Op OpAux Cks CESyn Syn)
+       (Import Typ   : NLTYPING        Ids Op OpAux Cks CESyn Syn Ord CETyp)
+       (Import DRR   : DUPREGREM       Ids Op OpAux Cks CESyn Syn).
+
+  Section substitute.
+    Variable sub : Env.t ident.
+
+    Variable inouts : list (ident * type).
+    Variable vars vars' : list (ident * type).
+
+    Hypothesis Hsub : forall x y ty,
+        Env.find x sub = Some y ->
+        In (x, ty) (inouts ++ vars) ->
+        In (y, ty) (inouts ++ vars').
+
+    Hypothesis Hnsub : forall x ty,
+        Env.find x sub = None ->
+        In (x, ty) (inouts ++ vars) ->
+        In (x, ty) (inouts ++ vars').
+
+    Lemma subst_in_var_wt : forall x ty,
+        In (x, ty) (inouts++vars) ->
+        In (subst_in_var sub x, ty) (inouts++vars').
+    Proof.
+      intros * Hin.
+      unfold subst_in_var.
+      destruct (Env.find _ _) eqn:Hfind; eauto.
+    Qed.
+
+    Variable (G : global).
+
+    Lemma subst_in_clock_wt : forall ck,
+        wt_clock G.(enums) (inouts++vars) ck ->
+        wt_clock G.(enums) (inouts++vars') (subst_in_clock sub ck).
+    Proof.
+      induction ck; intros * Hwt; inv Hwt; auto.
+      simpl. constructor; auto using subst_in_var_wt.
+    Qed.
+
+    Lemma subst_in_exp_wt : forall e,
+        wt_exp G.(enums) (inouts++vars) e ->
+        wt_exp G.(enums) (inouts++vars') (subst_in_exp sub e).
+    Proof.
+      intros * Hwt; induction Hwt;
+        simpl; econstructor; eauto using subst_in_var_wt.
+      1,2:repeat rewrite subst_in_exp_typeof; auto.
+    Qed.
+
+    Lemma subst_in_cexp_wt : forall e,
+        wt_cexp G.(enums) (inouts++vars) e ->
+        wt_cexp G.(enums) (inouts++vars') (subst_in_cexp sub e).
+    Proof.
+      induction e using cexp_ind2'; intros * Hwt; inv Hwt;
+        simpl; econstructor; eauto using subst_in_var_wt, subst_in_exp_wt.
+      1,5:rewrite map_length; auto.
+      - rewrite Forall_map. eapply Forall_impl; [|eapply H6]; intros.
+        rewrite subst_in_cexp_typeofc; auto.
+      - rewrite Forall_map. eapply Forall_impl_In; [|eapply H7]; intros.
+        eapply Forall_forall in H; eauto.
+      - rewrite subst_in_exp_typeof; eauto.
+      - intros.
+        eapply in_map_iff in H0 as (?&Hsome&Hin).
+        eapply option_map_inv in Hsome as (?&?&?); subst.
+        rewrite 2 subst_in_cexp_typeofc; auto.
+      - intros.
+        eapply in_map_iff in H0 as (?&Hsome&Hin).
+        eapply option_map_inv in Hsome as (?&?&?); subst.
+        eapply Forall_forall in H; eauto.
+        simpl in H; eauto.
+    Qed.
+
+    Hint Resolve subst_in_var_wt subst_in_clock_wt subst_in_exp_wt subst_in_cexp_wt.
+
+    Lemma subst_in_equation_wt : forall equ,
+        (forall x, In x (var_defined equ) -> Env.find x sub = None) ->
+        wt_equation G (inouts++vars) equ ->
+        wt_equation G (inouts++vars') (subst_in_equation sub equ).
+    Proof.
+      intros * Hdef Hwt; inv Hwt; simpl in *.
+      - constructor; auto.
+        rewrite subst_in_cexp_typeofc; auto.
+      - econstructor; eauto.
+        + eapply Forall2_impl_In; [|eauto]; intros ? (?&?&?) ? _ ?; auto.
+        + rewrite Forall2_map_1.
+          eapply Forall2_impl_In; [|eauto]; intros ? (?&?&?) _ _ Hty.
+          rewrite subst_in_exp_typeof; auto.
+        + rewrite Forall_map.
+          eapply Forall_impl_In; [|eapply H3]; intros; auto.
+        + rewrite Forall_map in *. unfold subst_in_reset.
+          rewrite Forall_map. eapply Forall_impl; [|eapply H4]; intros (?&?) (?&?).
+          simpl in *; eauto.
+        + rewrite Forall_map in *. unfold subst_in_reset.
+          rewrite Forall_map. eapply Forall_impl; [|eapply H5]; intros (?&?) ?.
+          simpl in *; auto.
+      - constructor; auto.
+        + rewrite subst_in_exp_typeof; auto.
+        + rewrite subst_in_exp_typeof; auto.
+        + rewrite Forall_map in *. unfold subst_in_reset.
+          rewrite Forall_map. eapply Forall_impl; [|eapply H3]; intros (?&?) (?&?).
+          simpl in *; eauto.
+        + rewrite Forall_map in *. unfold subst_in_reset.
+          rewrite Forall_map. eapply Forall_impl; [|eapply H4]; intros (?&?) ?.
+          simpl in *; auto.
+    Qed.
+
+  End substitute.
+
+  Lemma remove_dup_regs_once_wt : forall G inouts vars eqs,
+      NoDupMembers (inouts++idty vars) ->
+      NoDup (vars_defined eqs) ->
+      (forall x eq, In eq eqs -> In x (var_defined eq) -> is_fby eq = true -> ~InMembers x inouts) ->
+      Forall (wt_equation G (inouts++idty vars)) eqs ->
+      let (vars', eqs') := remove_dup_regs_eqs_once vars eqs in
+      Forall (wt_equation G (inouts++idty vars')) eqs'.
+  Proof.
+    intros * Hndv Hnd Hinouts Hwt.
+    destruct (remove_dup_regs_eqs_once _) eqn:Honce. inv Honce.
+    unfold subst_and_filter_equations.
+    rewrite Forall_map, Forall_filter. eapply Forall_impl_In; eauto.
+    intros ? Hineq Hwt' Hfilter.
+    eapply subst_in_equation_wt; [| | |eauto].
+    - intros * Hfind Hin.
+      assert (~InMembers x inouts) as Hnx.
+      { apply find_duplicates_spec in Hfind as (?&?&?&?&?&Hin1&_&_).
+        eapply Hinouts in Hin1; eauto. simpl; auto. }
+      assert (~InMembers y inouts) as Hny.
+      { apply find_duplicates_spec in Hfind as (?&?&?&?&?&_&Hin2&_).
+        eapply Hinouts in Hin2; eauto. simpl; auto. }
+      rewrite in_app_iff in *. destruct Hin as [Hin|Hin].
+      1:(exfalso; eauto using In_InMembers).
+      right.
+      rewrite In_idty_exists in *. destruct Hin as (?&Hin).
+      assert (Hfind':=Hfind).
+      eapply find_duplicates_spec in Hfind as (?&?&?&?&?&Hwt1&Hwt2&_).
+      eapply Forall_forall in Hwt1; eauto. eapply Forall_forall in Hwt2; eauto.
+      inv Hwt1. inv Hwt2.
+      rewrite in_app_iff in H4, H10.
+      destruct H4 as [Hin1|Hin1], H10 as [Hin2|Hin2].
+      1-3:(exfalso; eauto using In_InMembers).
+      eapply In_idty_exists in Hin1 as (?&Hin1).
+      eapply In_idty_exists in Hin2 as (ck&Hin2).
+      eapply NoDupMembers_det in Hin; eauto. 2:eapply NoDupMembers_app_r, NoDupMembers_idty in Hndv; eauto.
+      inv Hin. exists (subst_in_clock (find_duplicates eqs) ck); simpl.
+      unfold subst_and_filter_vars.
+      erewrite in_map_iff. exists (y, (typeof x3, ck)); split; auto.
+      eapply filter_In; split; auto.
+      eapply find_duplicates_irrefl in Hfind'; eauto.
+      apply Env.Props.P.F.not_mem_in_iff in Hfind'. rewrite Hfind'; auto.
+    - intros * Hfind Hin.
+      rewrite in_app_iff in *. destruct Hin as [Hin|Hin]; auto.
+      right.
+      rewrite In_idty_exists in *. destruct Hin as (ck&Hin).
+      exists (subst_in_clock (find_duplicates eqs) ck).
+      apply in_map_iff. exists (x, (ty, ck)); split; auto.
+      apply filter_In; split; auto.
+      rewrite Env.mem_find, Hfind; auto.
+    - intros * Hindef.
+      destruct (Env.find _ _) eqn:Hfind; auto. exfalso.
+      apply Env.find_In in Hfind.
+      assert (Hisfby:=Hindef). eapply find_duplicates_is_fby in Hisfby; eauto.
+      destruct a; simpl in *; try congruence.
+      inv Hindef; auto.
+      rewrite Bool.negb_true_iff, <-Env.Props.P.F.not_mem_in_iff in Hfilter.
+      congruence.
+  Qed.
+
+  Lemma remove_dup_regs_eqs_wt : forall G inouts vars eqs vars' eqs',
+      NoDupMembers (inouts ++ idty vars) ->
+      NoDup (vars_defined eqs) ->
+      (forall x eq, In eq eqs -> In x (var_defined eq) -> is_fby eq = true -> ~InMembers x inouts) ->
+      Forall (wt_equation G (inouts ++ idty vars)) eqs ->
+      remove_dup_regs_eqs vars eqs = (vars', eqs') ->
+      Forall (wt_equation G (inouts ++ idty vars')) eqs'.
+  Proof.
+    intros until eqs.
+    functional induction (remove_dup_regs_eqs vars eqs); intros * Hndv Hnd Hinouts Hwt Hrem.
+    - eapply remove_dup_regs_once_wt in Hwt; eauto.
+      rewrite e in Hwt. inv e.
+      eapply IHp; eauto using subst_and_filter_equations_NoDup.
+      + clear - Hndv.
+        apply NoDupMembers_app; eauto using NoDupMembers_app_l.
+        * apply NoDupMembers_app_r, NoDupMembers_idty in Hndv.
+          apply NoDupMembers_idty, subst_and_filter_vars_NoDupMembers; auto.
+        * intros ? Hin.
+          eapply NoDupMembers_app_InMembers in Hndv; eauto.
+          contradict Hndv.
+          rewrite InMembers_idty in *; eauto using subst_and_filter_vars_InMembers.
+      + intros ?? Hin1 Hin2 Hisfby.
+        eapply in_map_iff in Hin1 as (?&?&Hin1); subst. apply in_filter in Hin1.
+        destruct x0; simpl in *; try congruence. destruct Hin2 as [Hin2|Hin2]; inv Hin2.
+        eapply Hinouts; eauto. simpl; auto.
+    - inv Hrem; auto.
+  Qed.
+
+  Lemma remove_dup_regs_node_wt : forall G n,
+      wt_node G n ->
+      wt_node (remove_dup_regs G) (remove_dup_regs_node n).
+  Proof.
+    intros * (Hwteq&Henums).
+    constructor.
+    - simpl.
+      destruct (remove_dup_regs_eqs _ _) as (vars'&eqs') eqn:Hrem.
+      eapply remove_dup_regs_eqs_wt with (G:=G) (inouts:=idty (n_in n ++ n_out n)) (vars:=(n_vars n)) in Hrem; eauto.
+      + eapply Forall_impl; [|eauto]. intros ? Hwt.
+        eapply global_iface_eq_wt_eq; eauto using remove_dup_regs_iface_eq.
+        eapply wt_equation_incl; eauto. clear -n. intros ? Hin.
+        repeat rewrite idty_app in *. repeat rewrite <-filter_app in Hin.
+        repeat rewrite in_app_iff in *.
+        destruct Hin as [[Hin|Hin]|Hin]; auto.
+      + rewrite <-idty_app, <-app_assoc, (Permutation.Permutation_app_comm (n_out _)).
+        apply NoDupMembers_idty, n_nodup.
+      + apply NoDup_var_defined_n_eqs.
+      + intros. intros contra. rewrite idty_app, InMembers_app in contra. destruct contra as [contra|contra].
+        * rewrite InMembers_idty in contra.
+          assert (In x (vars_defined (n_eqs n))) as Hdef.
+          { unfold vars_defined. apply in_flat_map.
+            eexists; split; eauto. }
+          rewrite n_defd in Hdef. apply fst_InMembers in Hdef.
+          eapply NoDupMembers_app_InMembers in contra. eapply contra; eauto.
+          eapply n_nodup.
+        * rewrite fst_InMembers, map_fst_idty in contra.
+          apply n_vout in contra. apply contra.
+          unfold vars_defined. apply in_flat_map.
+          eexists; split; eauto.
+          apply filter_In; auto.
+      + eapply Forall_impl; [|eauto]. intros ? Hwt.
+        eapply wt_equation_incl; eauto. clear -n. intros (?&?) Hin.
+        rewrite <-idty_app, <-app_assoc, (Permutation.Permutation_app_comm (n_out _)).
+        assumption.
+    - intros; simpl in *. eapply Henums with (x:=x).
+      repeat rewrite idty_app, in_app_iff in *.
+      destruct H as [?|[Hin|?]]; auto.
+      right; left.
+      clear - Hin.
+      revert Hin.
+      functional induction (remove_dup_regs_eqs (n_vars n) (n_eqs n)); intros; auto.
+      apply IHp in Hin.
+      inv e. clear - Hin.
+      induction vars as [|(?&?&?)]; simpl in *; auto.
+      unfold subst_and_filter_vars in Hin; simpl in Hin.
+      destruct (negb _); simpl; auto.
+      inv Hin; auto.
+  Qed.
+
+  Theorem remove_dup_regs_wt : forall G,
+      wt_global G ->
+      wt_global (remove_dup_regs G).
+  Proof.
+    intros.
+    eapply CommonTyping.transform_units_wt_program; eauto.
+    intros. eapply remove_dup_regs_node_wt; eauto.
+  Qed.
+
+End DRRTYPING.
+
+Module DrrTypingFun
+       (Ids   : IDS)
+       (Op    : OPERATORS)
+       (OpAux : OPERATORS_AUX   Ids Op)
+       (Cks   : CLOCKS          Ids Op OpAux)
+       (CESyn : CESYNTAX        Ids Op OpAux Cks)
+       (CETyp : CETYPING        Ids Op OpAux Cks CESyn)
+       (Syn   : NLSYNTAX        Ids Op OpAux Cks CESyn)
+       (Ord   : NLORDERED       Ids Op OpAux Cks CESyn Syn)
+       (Typ   : NLTYPING        Ids Op OpAux Cks CESyn Syn Ord CETyp)
+       (DRR   : DUPREGREM       Ids Op OpAux Cks CESyn Syn)
+  <: DRRTYPING Ids Op OpAux Cks CESyn CETyp Syn Ord Typ DRR.
+  Include DRRTYPING Ids Op OpAux Cks CESyn CETyp Syn Ord Typ DRR.
+End DrrTypingFun.
